Weidenbach_Book/Prop_Superposition.thy
@@ -435,17 +435,17 @@ proof -
         f2: "\<forall>x0 x1. (\<exists>v2. v2 \<in> x0 \<and> Pos v2 \<notin> x1 \<and> Neg v2 \<notin> x1)
            \<longleftrightarrow> (aa x0 x1 \<in> x0 \<and> Pos (aa x0 x1) \<notin> x1 \<and> Neg (aa x0 x1) \<notin> x1)"
         by moura
-      have "\<forall>a. a \<notin> atms_of_m A \<or> Pos a \<in> I \<or> Neg a \<in> I"
+      have "\<forall>a. a \<notin> atms_of_ms A \<or> Pos a \<in> I \<or> Neg a \<in> I"
         using tot by (simp add: total_over_m_def total_over_set_def)
-      hence "aa (atms_of_m A \<union> atms_of_m {B}) (I \<union> {Pos a |a. a \<in> atms_of B \<and> a \<notin> atms_of_s I})
-        \<notin> atms_of_m A \<union> atms_of_m {B} \<or> Pos (aa (atms_of_m A \<union> atms_of_m {B})
+      hence "aa (atms_of_ms A \<union> atms_of_ms {B}) (I \<union> {Pos a |a. a \<in> atms_of B \<and> a \<notin> atms_of_s I})
+        \<notin> atms_of_ms A \<union> atms_of_ms {B} \<or> Pos (aa (atms_of_ms A \<union> atms_of_ms {B})
           (I \<union> {Pos a |a. a \<in> atms_of B \<and> a \<notin> atms_of_s I})) \<in> I
             \<union> {Pos a |a. a \<in> atms_of B \<and> a \<notin> atms_of_s I}
-          \<or> Neg (aa (atms_of_m A \<union> atms_of_m {B})
+          \<or> Neg (aa (atms_of_ms A \<union> atms_of_ms {B})
             (I \<union> {Pos a |a. a \<in> atms_of B \<and> a \<notin> atms_of_s I})) \<in> I
             \<union> {Pos a |a. a \<in> atms_of B \<and> a \<notin> atms_of_s I}"
         by auto
-      hence "total_over_set (I \<union> {Pos a |a. a \<in> atms_of B \<and> a \<notin> atms_of_s I}) (atms_of_m A \<union> atms_of_m {B})"
+      hence "total_over_set (I \<union> {Pos a |a. a \<in> atms_of B \<and> a \<notin> atms_of_s I}) (atms_of_ms A \<union> atms_of_ms {B})"
         using f2 by (meson total_over_set_def)
       thus ?thesis
         by (simp add: total_over_m_def)
